\section*{1.4.2}
For events $A_1$, $A_2$, $\ldots$, $A_n$ satisfying
$P(A_1\cap A_2\cap\cdots\cap A_{n-1})>0$,
prove that
\begin{eqnarray*}
\lefteqn{P(A_1\cap A_2\cap\cdots\cap A_{n-1})}\\
&&=P(A_1)P(A_2\mid A_1)P(A_3\mid A_1\cap A_2)\cdots
P(A_n\mid A_1\cap A_2\cap\cdots\cap A_{n-1})
\end{eqnarray*}

\bigskip
\noindent
For $n=1$ we have
$$P(A_1)=P(A_1)$$
For $n=2$ we have
$$P(A_1\cap A_2)=P(A_1)P(A_2\mid A_1)$$
which is the definition of conditional probability.
For $n=3$ note that
$$P(A_3\mid A_1\cap A_2)={P(A_1\cap A_2\cap A_3)\over P(A_1\cap A_2)}$$
hence
\begin{eqnarray*}
P(A_1\cap A_2\cap A_3)&=&P(A_1\cap A_2)P(A_3\mid A_1\cap A_2)\\
&=&P(A_1)P(A_2\mid A_1)P(A_3\mid A_1\cap A_2)
\end{eqnarray*}
For the induction step, assume the equation is true for $n$.
Then for $n+1$ we have
$$P(A_{n+1}\mid A_1\cap A_2\cap\cdots\cap A_n)=
{P(A_1\cap A_2\cap\cdots\cap A_{n+1})\over
P(A_1\cap A_2\cap\cdots\cap A_n)}$$
Hence
\begin{eqnarray*}
\lefteqn{P(A_1\cap A_2\cap\cdots\cap A_{n+1})}\\
&&=
P(A_1\cap A_2\cap\cdots\cap A_n)
P(A_{n+1}\mid A_1\cap A_2\cap\cdots\cap A_n)\\
&&=P(A_1)P(A_2\mid A_1)P(A_3\mid A_1\cap A_2)\cdots
P(A_{n+1}\mid A_1\cap A_2\cap\cdots\cap A_n)
\end{eqnarray*}
This proves the equation is true for $n+1$ whenever it is true for
$n$.
Therefore by induction, it is true for all $n\in N$.

