\section*{4.7.5}
Let $X$ and $Y$ have the bivariate normal density function
$$f(x,y)={1\over2\pi\sqrt{1-\rho^2}}
\exp\left\{
-{1\over2(1-\rho^2)}(x^2-2\rho xy+y^2)\right\}$$
Show that $X$ and $Z=(Y-\rho X)/\sqrt{1-\rho^2}$ are independent
$N(0,1)$ variables, and deduce that
$$P(X>0,Y>0)={1\over4}+{1\over2\pi}\sin^{-1}\rho$$

\bigskip
\noindent
We have
$$\left(\matrix{
X\cr
Y}\right)
\sim N\left(
\left(\matrix{
0\cr
0}\right),
\left(\matrix{
1 & \rho\cr
\rho & 1}\right)\right)
$$
Let
$$\Sigma=\left(\matrix{
1 & \rho\cr
\rho & 1
}\right)
$$
$$B=\left(\matrix{-{\rho\over\sqrt{1-\rho^2}}
& {1\over\sqrt{1-\rho^2}}}\right)$$
Then
$$Z=B\left(\matrix{
X\cr
Y}\right)
\sim N(0,B\Sigma B^T)=N(0,1)
$$
Hence $Z\sim N(0,1)$. Let
$$B=\left(\matrix{
1 & 0 \cr
-{\rho\over\sqrt{1-\rho^2}} & {1\over\sqrt{1-\rho^2}}
}\right)$$
Then
$$\left(\matrix{X\cr Z}\right)
=
B\left(\matrix{X\cr Y}\right)
=N(0,B\Sigma B^T)=
N\left(
\left(\matrix{0\cr 0}\right),
\left(\matrix{
1 & 0\cr
0 & 1
}\right)\right)
$$
Since the covariant terms are 0, $X$ and $Z$ are independent.

\bigskip
\noindent
For $P(X>0,Y>0)$ we need $f_{XZ}(x,z)$.
For the inverse transform we have
\begin{eqnarray*}
X&=&X\\
Y&=&\sqrt{1-\rho^2}Z+\rho X
\end{eqnarray*}
Hence
$$J_{T^{-1}}=\left(\matrix{
\partial X/\partial X & \partial X/\partial Z\cr\cr
\partial Y/\partial X & \partial Y/\partial Z
}\right)
=\left(\matrix{
1 & 0\cr\cr
\rho & \sqrt{1-\rho^2}
}\right)
$$
Therefore
$$|\det J_{T^{-1}}|=\sqrt{1-\rho^2}$$
We have
\begin{eqnarray*}
f_{XZ}(x,z)&=&f(x,\sqrt{1-\rho^2}z+\rho x)\cdot\sqrt{1-\rho^2}\\
&=&{1\over2\pi}\exp\left(-{x^2\over2}-{z^2\over2}\right)
\end{eqnarray*}
Since $Y=\sqrt{1-\rho^2}Z+\rho X$ we have
$$P(X>0,Y>0)=P(X>0,Z>-\rho X/\sqrt{1-\rho^2})$$
Changing to polar coordinates we have
$$\alpha=\tan^{-1}{z\over x}
=\tan^{-1}{-\rho x/\sqrt{1-\rho^2}\over x}
=-\tan^{-1}{\rho\over\sqrt{1-\rho^2}}=-\sin^{-1}\rho$$
Hence
\begin{eqnarray*}
P(X>0,Y>0)
&=&{1\over2\pi}\int_\alpha^{\pi/2}
\int_0^\infty
\exp(-r^2/2)\,r\,dr\,d\theta\\
&=&{1\over2\pi}
\int_\alpha^{\pi/2}\left(-\exp(-r^2/2)\bigg|_0^\infty\right)
\,d\theta\\
&=&{1\over2\pi}\int_\alpha^{\pi/2}d\theta\\
&=&{1\over2\pi}\left({\pi\over2}+\sin^{-1}\rho\right)\\
&=&{1\over4}+{1\over2\pi}\sin^{-1}\rho
\end{eqnarray*}
