\section*{4.7.14}
Let $X$ and $Y$ be independent and gamma distributed as
$\Gamma(\lambda,\alpha)$, $\Gamma(\lambda,\beta)$ respectively.
Show that $W=X+Y$ and $Z=X/(X+Y)$ are independent, and that
$Z$ has the beta distribution with parameters $\alpha$, $\beta$.

\bigskip
\noindent
The joint density of $X$ and $Y$ is
$$f_{XY}(x,y)=
\left({1\over\Gamma(\alpha)}\lambda^\alpha x^{\alpha-1}
e^{-\lambda x}\right)
\left({1\over\Gamma(\beta)}\lambda^\beta x^{\beta-1}
e^{-\lambda x}\right)
$$
The inverse transform is
$$x=wz,\quad y=w-wz$$
The Jacobian transform is
$$J_{T^{-1}}=\left(\matrix{
\partial x/\partial w & \partial x/\partial z\cr
\partial y/\partial w & \partial y/\partial z
}\right)
=\left(\matrix{
z & w\cr
1-z & -w
}\right)$$
%
The absolute value of the determinant of the Jacobian is
$$|\det J_{T^{-1}}|=|-wz-w(1-z)|=|w|=w$$
We can drop the absolute value because the domain of $X$ and $Y$
is $[0,\infty)$ hence $w$ is nonnegative.
Put it all together
\begin{eqnarray*}
f_{WZ}(w,z)&=&f_{XY}(wz,w(1-z))\cdot w\\
&=&
\left({1\over\Gamma(\alpha)}\lambda^\alpha (wz)^{\alpha-1}
e^{-\lambda wz}\right)
\left({1\over\Gamma(\beta)}\lambda^\beta
(w(1-z))^{\beta-1}e^{-\lambda w(1-z)}\right)w\\
&=&f_W(w)f_Z(z)
\end{eqnarray*}
where
$$f_W(w)={1\over\Gamma(\alpha+\beta)}\lambda^{\alpha+\beta}
w^{\alpha+\beta-1}e^{-\lambda w}$$
and
$$f_Z(z)={\Gamma(\alpha+\beta)\over\Gamma(\alpha)\Gamma(\beta)}
z^{\alpha-1}(1-z)^{\beta-1}$$
Hence $W$ and $Z$ are independent and $Z\sim Beta(\alpha,\beta)$.
