\section*{4.9.6}
Let $\{Y_r:1\le r\le n\}$ be independent $N(0,1)$ random variables,
and define $X_j=\sum_{r=1}^n c_{jr}Y_r$,
$1\le r\le n$, for constants $c_{jr}$. Show that
$$E(X_j\mid X_k)=\left(\sum_r c_{jr}c_{kr}\over\sum_r c_{kr}^2\right)
X_k$$

\bigskip
\noindent
It turns out that
$$E(X_j\mid X_k)={\mathop{Cov}(X_j,X_k)\over\mathop{Var}X_k}X_k$$
which I will prove later.
Let $C$ be the coefficient matrix such that
$$X=CY$$
Then the covariance matrix $A$ is
$$A=CC^T$$
We have
$$\mathop{Cov}(X_j,X_k)=A_{jk}=
(\hbox{row $j$ of $C$})
(\hbox{column $k$ of $C^T$})
=\sum_r c_{jr}c_{kr}$$
and
$$\mathop{Var}X_k=A_{kk}=
(\hbox{row $k$ of $C$})
(\hbox{column $k$ of $C^T$})
=\sum_r c_{kr}^2$$
Hence
$$E(X_j\mid X_k)=\left(\sum_r c_{jr}c_{kr}\over\sum_r c_{kr}^2\right)
X_k$$
%
Now for the proof that
$$E(Y\mid X)={\mathop{Cov}(X,Y)\over\mathop{Var}X}X$$
for $X\sim N(0,\sigma_X^2)$ and $Y\sim N(0,\sigma_Y^2)$.
We have
$$f_{XY}(x,y)={1\over2\pi\sigma_X\sigma_Y\sqrt{1-\rho^2}}
\exp\left[
-{1\over2(1-\rho^2)}
\left(
{x^2\over\sigma_X^2}
-{2\rho xy\over\sigma_X\sigma_Y}
+{y^2\over\sigma_Y^2}
\right)\right]
$$
and
$$f_{X}(x)={1\over\sqrt{2\pi}\sigma_X}
\exp\left(-{x^2\over2\sigma_X^2}\right)$$
Hence
\begin{eqnarray*}
f_{Y\mid X}(y\mid x)
&=&{f_{XY}(x,y)\over f_X(x)}\\
&=&{1\over\sqrt{2\pi}\sigma_Y\sqrt{1-\rho^2}}
\exp\left[-{1\over2(1-\rho^2)}\left(
{x^2\over\sigma_X^2}
-{2\rho xy\over\sigma_X\sigma_Y}
+{y^2\over\sigma_Y^2}
-{(1-\rho^2)x^2\over\sigma_X^2}
\right)\right]\\
%
&=&{1\over\sqrt{2\pi}\sigma_Y\sqrt{1-\rho^2}}
\exp\left[-{1\over2(1-\rho^2)}\left(
{\rho^2x^2\over\sigma_X^2}
-{2\rho xy\over\sigma_X\sigma_Y}
+{y^2\over\sigma_Y^2}
\right)\right]\\
%
&=&{1\over\sqrt{2\pi}\sigma_Y\sqrt{1-\rho^2}}
\exp\left[-{1\over2\sigma_Y^2(1-\rho^2)}\left(
{\sigma_Y^2\rho^2x^2\over\sigma_X^2}
-{2\sigma_Y\rho xy\over\sigma_X}
+y^2
\right)\right]\\
%
&=&{1\over\sqrt{2\pi}\sigma_Y\sqrt{1-\rho^2}}
\exp\left[-{1\over2\sigma_Y^2(1-\rho^2)}\left(
y-{\sigma_Y\rho x\over\sigma_X}\right)^2\right]
\end{eqnarray*}
Therefore
$$(Y\mid X=x)\sim N\left(
{\sigma_Y\rho x\over\sigma_X},\sigma_Y^2(1-\rho^2)\right)$$
Hence
$$E(Y\mid X)={\sigma_Y\rho\over\sigma_X}X
={\mathop{Cov}(X,Y)\over\mathop{Var}X}X$$
