\section*{4.9.9}
Let $X$, $Y$, $Z$ have the standard trivariate normal
density of Exercise
(8), with $\rho_1=\rho(X,Y)$. Show that
\begin{eqnarray*}
E(Z\mid X,Y)&=&
\left[(\rho_2-\rho_1\rho_3)X+(\rho_3-\rho_1\rho_2)Y\right]
/(1-\rho_1^2)\\
%
\mathop{Var}(Z\mid X,Y)&=&
\left[1-\rho_1^2-\rho_2^2-\rho_3^2+2\rho_1\rho_2\rho_3\right]
/(1-\rho_1^2)
\end{eqnarray*}

\bigskip
\noindent
The typo in the expectation has been corrected above.
Let $A$ and $B$ be the following covariance matrices.
$$A=\left(\matrix{
1 & \rho_1 & \rho_2 \cr
\rho_1 & 1 & \rho_3 \cr
\rho_2 & \rho_3 & 1
}\right)\qquad
B=\left(\matrix{
1 & \rho_1 \cr
\rho_1 & 1
}\right)
$$
Then
$$A^{-1}={1\over\det A}\mathop{\rm adj}A
\qquad\det A=1-\rho_1^2-\rho_2^2-\rho_3^2+2\rho_1\rho_2\rho_3
$$
$$
\mathop{\rm adj}A=\left(\matrix{
1-\rho_3^2 & \rho_2\rho_3-\rho_1 & \rho_1\rho_3-\rho_2 \cr
\rho_2\rho_3-\rho_1 & 1-\rho_2^2 & \rho_1\rho_2-\rho_3 \cr
\rho_1\rho_3-\rho_2 & \rho_1\rho_2-\rho_3 & 1-\rho_1^2
}\right)$$
and
$$B^{-1}={1\over\det B}\mathop{\rm adj}B
\qquad\det B=1-\rho_1^2\qquad
\mathop{\rm adj}B=\left(\matrix{
1 & -\rho_1 \cr
-\rho_1 & 1
}\right)$$
Let $X=(x,y,z)$ and $Y=(x,y)$. Then
$$f_{XYZ}(x,y,z)={1\over\sqrt{(2\pi)^3\det A}}\exp\left[
-{1\over2\det A}X^T(\mathop{\rm adj}A)X\right]$$
and
$$f_{XY}(x,y)={1\over\sqrt{(2\pi)^2\det B}}\exp\left[
-{1\over2\det B}Y^T(\mathop{\rm adj}B)Y\right]$$
Therefore
\begin{eqnarray*}
f_{Z\mid X,Y}(z\mid x,y)&=&
{f_{XYZ}(x,y,z)\over f_{XY}(x,y)}\\
&=&{1\over\sqrt{2\pi\det A/\det B}}\exp\left[
-{X^T(\mathop{\rm adj}A)X\over2\det A}
+{Y^T(\mathop{\rm adj}B)Y\over2\det B}
\right]
\end{eqnarray*}
We have immediately that
$$\sigma^2={\det A\over\det B}
={1-\rho_1^2-\rho_2^2-\rho_3^2+2\rho_1\rho_2\rho_3
\over1-\rho_1^2}$$
Let
$$P=(\det B)X^T(\mathop{\rm adj}A)X
-(\det A)Y^T(\mathop{\rm adj}B)Y$$
Then
$$f_{Z\mid X,Y}(z\mid x,y)=
{1\over\sqrt{2\pi\det A/\det B}}\exp\left[
-{P\over2\det A\det B}\right]$$
We have
\begin{eqnarray*}
P&=&-2\rho_1\rho_2\rho_3x^2-2\rho_1\rho_2\rho_3y^2+2\rho_1\rho_2yz\\
& & {}+2\rho_1\rho_3xz-2\rho_1\rho_2^2xy-2\rho_1\rho_3^2xy\\
& & {}+2\rho_2\rho_3xy-2\rho_2xz-2\rho_3yz\\
& & {}+z^2+2\rho_1^2\rho_2\rho_3xy+2\rho_1^2\rho_2xz\\
& & {}+2\rho_1^2\rho_3yz+\rho_1^2\rho_2^2y^2+\rho_1^2\rho_3^2x^2\\
& & {}-2\rho_1^2z^2-2\rho_1^3\rho_2yz-2\rho_1^3\rho_3xz\\
& & {}+\rho_1^4z^2+\rho_2^2x^2+\rho_3^2y^2
\end{eqnarray*}
Let
$$\mu={(\rho_2-\rho_1\rho_3)x+(\rho_3-\rho_1\rho_2)y\over
1-\rho_1^2}$$
We want to show that
$$f_{Z\mid X,Y}(z\mid x,y)=
{1\over\sqrt{2\pi\det A/\det B}}\exp\left[
-{\det B\over2\det A}(z-\mu)^2\right]$$
Let
$$Q=[\det B(z-\mu)]^2$$
Then
$$-{\det B\over2\det A}(z-\mu)^2=-{Q\over2\det A\det B}$$
We have
\begin{eqnarray*}
Q&=&-2\rho_1\rho_2\rho_3x^2-2\rho_1\rho_2\rho_3y^2+2\rho_1\rho_2yz\\
& & {}+2\rho_1\rho_3xz-2\rho_1\rho_2^2xy-2\rho_1\rho_3^2xy\\
& & {}+2\rho_2\rho_3xy-2\rho_2xz-2\rho_3yz\\
& & {}+z^2+2\rho_1^2\rho_2\rho_3xy+2\rho_1^2\rho_2xz\\
& & {}+2\rho_1^2\rho_3yz+\rho_1^2\rho_2^2y^2+\rho_1^2\rho_3^2x^2\\
& & {}-2\rho_1^2z^2-2\rho_1^3\rho_2yz-2\rho_1^3\rho_3xz\\
& & {}+\rho_1^4z^2+\rho_2^2x^2+\rho_3^2y^2
\end{eqnarray*}
hence $P=Q$ and the mean is indeed $\mu$.
