\section*{1.4.6}
Let $G$ be the event that an accused is guilty, and $T$ the event that
some testimony is true.
Some lawyers have argued on the assumption that
$P(G\mid T)=P(T\mid G)$.
Show that this holds if and only if $P(G)=P(T)$.

\bigskip
\noindent
First show the implication.
Let
$$P(G\mid T)=P(T\mid G)$$
Then
$${P(G\cap T)\over P(T)}={P(G\cap T)\over P(G)}$$
hence
$$P(G)=P(T)$$
Now show the converse. Let
$$P(G)=P(T)$$
Then
$${P(G\cap T)\over P(T)}={P(G\cap T)\over P(G)}$$
hence
$$P(G\mid T)=P(T\mid G)$$
Therefore $P(G\mid T)=P(T\mid G)$ if and only if
$P(G)=P(T)$.

