\section*{4.6.2}
Show that the conditional expectation $\psi(X)=E(Y\mid X)$
satisfies $E(\psi(X)g(X))=E(Yg(X))$, for any function $g$
for which both expectations exist.

\bigskip
\noindent
See lecture \#26. We have
\begin{eqnarray*}
E(\psi(X)g(X))
&=&\int_{-\infty}^{\infty}
E(Y\mid X=x)g(x)f_X(x)\,dx\\
&=&\int_{-\infty}^\infty
\left(\int_{-\infty}^\infty y{f_{XY}(x,y)\over f_X(x)}\,dy\right)
g(x)f_X(x)\,dx\\
&=&\int_{-\infty}^\infty\int_{-\infty}^\infty
yg(x)f_{XY}(x,y)\,dx\,dy\\
&=&E(Yg(X))
\end{eqnarray*}
