\section*{4.5.5}
Let $X$ and $Y$ be independent continuous random variables.
Show that
$$E(g(X)h(Y))=E(g(X))E(h(Y))$$
whenever these expectations exist.
If $X$ and $Y$ have the exponential distribution with parameter 1,
find $E[\exp({1\over2}(X+Y))]$.

\begin{eqnarray*}
E(g(x)h(y))
&=&\int_{-\infty}^\infty\int_{-\infty}^\infty
g(x)f_X(x)h(y)f_Y(y)\,dx,dy\\
&=&\int_{-\infty}^\infty
g(x)f_X(x)\,dx\left(
\int_{-\infty}^\infty h(y)f_Y(y)\,dy\right)\\
&=&\int_{-\infty}^\infty g(x)f_X(x)\,dx\cdot E(h(Y))\\
&=&E(g(X))E(h(Y))
\end{eqnarray*}

\bigskip
\noindent
For $E[\exp({1\over2}(X+Y))]$ we have
$$f_X(x)=e^{-x},\quad f_Y(y)=e^{-y},\quad f(x,y)=f_X(x)f_Y(y)
=e^{-x}e^{-y}$$
$$g(x,y)=\exp((x+y)/2)=e^{x/2}e^{y/2}$$
\begin{eqnarray*}
E[\exp((X+Y)/2)]
&=&\int_0^\infty\int_0^\infty g(x,y)f(x,y)\,dx\,dy\\
&=&\int_0^\infty\int_0^\infty e^{x/2}e^{y/2}e^{-x}e^{-y}\,dx\,dy\\
&=&\left(\int_0^\infty e^{-x/2}\,dx\right)
\left(\int_0^\infty e^{-y/2}\,dy\right)\\
&=&\left(-2e^{-x/2}\bigg|_0^\infty\right)
\left(-2e^{-y/2}\bigg|_0^\infty\right)\\
&=&4
\end{eqnarray*}
