\section*{3.6.8}
Let $X$ and $Y$ have joint mass function
$$f(j,k)={c(j+k)a^{j+k}\over j!\,k!},\quad j,k\ge0$$
where $a$ is a constant.
Find $c$, $P(X=j)$, $P(X+Y=r)$, and $E(X)$.

\bigskip
\noindent
For $c$ we have
\begin{eqnarray*}
\sum_{j,k}f(j,k)
&=&c\left[
\sum_{j=0}^\infty{ja^j\over j!}
\left(\sum_{k=0}^\infty{a^k\over k!}\right)
+
\sum_{k=0}^\infty{ka^k\over k!}
\left(\sum_{j=0}^\infty{a^j\over j!}\right)
\right]\\
%
&=&c\left[
\sum_{j=0}^\infty{ja^j\over j!}e^a
+
\sum_{k=0}^\infty{ka^k\over k!}e^a
\right]\\
%
&=&c\left[
\sum_{j=1}^\infty{ja^j\over j!}e^a
+
\sum_{k=1}^\infty{ka^k\over k!}e^a
\right]\\
%
&=&c\left[
a\sum_{j=1}^\infty{a^{j-1}\over(j-1)!}e^a
+
a\sum_{k=1}^\infty{a^{k-1}\over(k-1)!}e^a
\right]\\
&=&c(ae^ae^a+ae^ae^a)\\
&=&c\cdot2ae^{2a}
\end{eqnarray*}
Therefore
$$c={1\over2ae^{2a}}$$

\bigskip
\noindent
For $P(X=j)$ we have
\begin{eqnarray*}
\sum_k f(j,k)
&=&{1\over2ae^{2a}}
\left({ja^j\over j!}\sum_{k=0}^\infty{a^k\over k!}
+{a^j\over j!}\sum_{k=0}^\infty{ka^k\over k!}\right)\\
&=&{1\over2ae^{2a}}\left(
{ja^j\over j!}e^a+{a^j\over j!}ae^a
\right)\\
%&=&{1\over2e^a}\left({a^j\over j!}+{a^{j-1}\over(j-1)!}\right)
&=&{1\over2e^a}\left({ja^{j-1}+a^j\over j!}\right)
\end{eqnarray*}

\bigskip
\noindent
For $P(X+Y=r)$ we have
\begin{eqnarray*}
\sum_j f(j,r-j)
&=&{1\over 2ae^{2a}}\sum_{j=0}^\infty
{(j+r-j)a^{j+r-j}\over j!\,(r-j)!}\\
&=&{1\over2ae^{2a}}\cdot
{ra^r\over r!}\sum_{j=0}^\infty{r!\over j!\,(r-j)!}\\
&=&{1\over2ae^{2a}}\cdot{ra^r\over r!}\cdot2^r
\end{eqnarray*}

\bigskip
\noindent
For $E(X)$ we have
\begin{eqnarray*}
\sum_{j,k}jf(j,k)
&=&{1\over2ae^{2a}}\left[
\sum_{j=0}^\infty{j^2a^j\over j!}
\left(\sum_{k=0}^\infty{a^k\over k!}\right)
+
\sum_{j=0}^\infty{ja^j\over j!}
\left(\sum_{k=0}^\infty{ka^k\over k!}\right)
\right]\\
%
&=&{1\over2ae^{2a}}\left[
\sum_{j=0}^\infty{j^2a^j\over j!}e^a
+
a^2e^{2a}
\right]\\
%
&=&{1\over2ae^{2a}}\left[
a\sum_{j=1}^\infty{ja^{j-1}\over(j-1)!}e^a+a^2e^{2a}
\right]\\
%
&=&{1\over2ae^{2a}}\left[
a\sum_{j=0}^\infty{(j+1)a^j\over j!}e^a+a^2e^{2a}
\right]\\
%
&=&{1\over2ae^{2a}}\left[
a(ae^a+e^a)e^a+a^2e^{2a}
\right]\\
%
&=&{1\over2ae^{2a}}\left[
a^2e^{2a}+ae^{2a}+a^2e^{2a}\right]\\
%
&=&{2a^2e^{2a}+ae^{2a}\over2ae^{2a}}\\
&=&a+{1\over2}
\end{eqnarray*}
