\section{Section 25.5, problem 7}
Let $\bf A$ be an $n\times n$ matrix for which ${\bf I}_n-{\bf A}$
is nonsingular.
If $\lambda$ is an eigenvalue of $\bf A$ show that $(1-\lambda)^{-1}$
is an eigenvalue of $({\bf I}_n-{\bf A})^{-1}$.

\bigskip
\noindent
Let $\vec x$ be the eigenvector associated with $\lambda$.
Theorem 9.4 tells us that ${\bf C}^{-1}{\bf AC}x=\lambda x$ for any
nonsingular matrix $\bf C$. Therefore we can write
$$({\bf I}_n-{\bf A})^{-1}{\bf A}({\bf I}_n-{\bf A})\vec x
=\lambda\vec x$$
Note that
\begin{eqnarray*}
({\bf I}_n-{\bf A})^{-1}{\bf A}({\bf I}_n-{\bf A})\vec x
&=&({\bf I}_n-{\bf A})^{-1}({\bf A}-{\bf A}^2)\vec x\\
&=&({\bf I}_n-{\bf A})^{-1}({\bf A}\vec x-{\bf A}^2\vec x)\\
&=&({\bf I}_n-{\bf A})^{-1}(\lambda\vec x-\lambda^2\vec x)\\
&=&({\bf I}_n-{\bf A})^{-1}(\lambda-\lambda^2)\vec x
\end{eqnarray*}
It follows that
$$({\bf I}_n-{\bf A})^{-1}(\lambda-\lambda^2)\vec x=\lambda\vec x$$
Hence
$$({\bf I}_n-{\bf A})^{-1}\vec x
={\lambda\over\lambda-\lambda^2}\,\vec x={1\over1-\lambda}\,\vec x$$
Therefore $(1-\lambda)^{-1}$ is an eigenvalue of
$({\bf I}_n-{\bf A})^{-1}$.
