\section{Section 25.3, problem 5}
Show that $\bf G$ is the inverse of $\bf X$.
We have
\begin{eqnarray*}
{\bf X}_{11}{\bf G}_{11}&=&{\bf I}+{\bf X}_{12}{\bf X}_{22\cdot1}^{-1}{\bf X}_{21}{\bf X}_{11}^{-1}\\
{\bf X}_{12}{\bf G}_{21}&=&-{\bf X}_{12}{\bf X}_{22\cdot1}^{-1}{\bf X}_{21}{\bf X}_{11}^{-1}\\
\\
{\bf X}_{11}{\bf G}_{12}&=&-{\bf X}_{12}{\bf X}_{22\cdot1}^{-1}\\
{\bf X}_{12}{\bf G}_{22}&=&{\bf X}_{12}{\bf X}_{22\cdot1}^{-1}\\
\\
{\bf X}_{21}{\bf G}_{11}&=&{\bf X}_{21}{\bf X}_{11}^{-1}+
{\bf X}_{21}{\bf X}_{11}^{-1}{\bf X}_{12}{\bf X}_{22\cdot1}^{-1}{\bf X}_{21}{\bf X}_{11}^{-1}\\
{\bf X}_{22}{\bf G}_{21}&=&-{\bf X}_{22}{\bf X}_{22\cdot1}^{-1}{\bf X}_{21}{\bf X}_{11}^{-1}\\
\\
{\bf X}_{21}{\bf G}_{12}&=&-{\bf X}_{21}{\bf X}_{11}^{-1}{\bf X}_{12}{\bf X}_{22\cdot1}^{-1}\\
{\bf X}_{22}{\bf G}_{22}&=&{\bf X}_{22}{\bf X}_{22\cdot1}^{-1}
\end{eqnarray*}
Hence
\begin{eqnarray*}
{\bf X}_{11}{\bf G}_{11}+{\bf X}_{12}{\bf G}_{21}&=&{\bf I}\\
\\
{\bf X}_{11}{\bf G}_{11}+{\bf X}_{12}{\bf G}_{22}&=&{\bf 0}\\
\\
{\bf X}_{21}{\bf G}_{11}+{\bf X}_{22}{\bf G}_{21}&=&{\bf X}_{21}{\bf X}_{11}^{-1}+
({\bf X}_{21}{\bf X}_{11}^{-1}{\bf X}_{12}-{\bf X}_{22}){\bf X}_{22\cdot1}^{-1}{\bf X}_{21}{\bf X}_{11}^{-1}\\
&=&{\bf X}_{21}{\bf X}_{11}^{-1}-{\bf X}_{22\cdot1}{\bf X}_{22\cdot1}^{-1}{\bf X}_{21}{\bf X}_{11}^{-1}\\
&=&{\bf 0}\\
\\
{\bf X}_{21}{\bf G}_{12}+{\bf X}_{22}{\bf G}_{22}&=&-{\bf X}_{21}{\bf X}_{11}^{-1}{\bf X}_{12}{\bf X}_{22\cdot1}^{-1}
+{\bf X}_{22}{\bf X}_{22\cdot1}^{-1}\\
&=&{\bf X}_{22\cdot1}{\bf X}_{22}^{-1}\\
&=&{\bf I}
\end{eqnarray*}
Therefore
$$\left(\begin{matrix}
{\bf X}_{11} & {\bf X}_{12}\cr
{\bf X}_{21} & {\bf X}_{22}
\end{matrix}\right)\left(\begin{matrix}
{\bf G}_{11} & {\bf G}_{12}\cr
{\bf G}_{21} & {\bf G}_{22}
\end{matrix}\right)=\left(\begin{matrix}
{\bf I} & {\bf 0}\cr
{\bf 0} & {\bf I}
\end{matrix}\right)
$$
