\section*{26.4.1}
Let
$${\bf A}=\left(\begin{matrix}
1 & 0\cr
0 & 0
\end{matrix}\right)
$$
Find a non-symmetric generalized inverse of {\bf A}.

\bigskip
\noindent
Note that ${\bf{AAA}=A}$ hence ${\bf A}$ is a generalized inverse
of itself.
Let
$${\bf G}=\left(\begin{matrix}
1 & 0\cr
0 & 0
\end{matrix}\right),\quad
{\bf S}=\left(\begin{matrix}
s_{11} & s_{12}\cr
s_{21} & s_{22}
\end{matrix}\right),\quad
{\bf T}=\left(\begin{matrix}
t_{11} & t_{12}\cr
t_{21} & t_{22}
\end{matrix}\right)
$$
Then
$${\bf G}^*={\bf GAG}+{\bf S}({\bf I}-{\bf AG})
+({\bf I}-{\bf GA}){\bf T}
=\left(\begin{matrix}
1 & s_{12}\cr
t_{21} & s_{22}+t_{22}
\end{matrix}\right)
$$
It follows that ${\bf G}^*$ is a generalized inverse of $\bf A$ for
all values of $s_{12}$, $t_{21}$, and $s_{22}+t_{22}$.
Hence
$${\bf A}^{-{}}=\left(\begin{matrix}
1 & 1\cr
0 & 0
\end{matrix}\right)
$$
is a non-symmetric generalized inverse of $\bf A$.
