\documentclass[12pt]{article}
\usepackage{amsmath}
\parindent=0pt
\begin{document}

(2.2)
For the Hamiltonian
$\hat H=\frac{\hat p^2}{2m}+\frac{1}{2}m\omega^2\hat x^2+\lambda\hat x^4$,
where $\lambda$ is small, show by writing the Hamiltonian
in terms of creation and annihilation operators and
using perturbation theory, that the energy eigenvalues
of all the levels are given by
\begin{equation*}
E_n=\left(n+\frac{1}{2}\right)\hbar\omega
+\frac{3\lambda}{4}\left(\frac{\hbar}{m\omega}\right)^2
\left(2n^2+2n+1\right)
\tag{2.67}
\end{equation*}

\bigskip
\hrule

\bigskip
Consider equations (2.12) and (2.14).
\begin{align*}
\hat x&=\sqrt{\frac{\hbar}{2m\omega}}\left(\hat a+\hat a^\dag\right)
\tag{2.12}
\\
\hat H&=\hbar\omega\left(\hat a^\dag\hat a+\frac{1}{2}\right)
\tag{2.14}
\end{align*}

Then the Hamiltonian for this problem is
\begin{equation*}
\hat H=\hbar\omega\left(\hat a^\dag\hat a+\frac{1}{2}\right)
+\lambda\left(\sqrt{\frac{\hbar}{2m\omega}}\left(\hat a+\hat a^\dag\right)\right)^4
\tag{1}
\end{equation*}

Noting that
\begin{equation*}
\left(\hat a+\hat a^\dag\right)^2
=\hat a\hat a^\dag+\hat a^\dag\hat a
\end{equation*}
we have by the commutator $\hat a\hat a^\dag-\hat a^\dag\hat a=1$ that
\begin{equation*}
\left(\hat a+\hat a^\dag\right)^2
=(1+\hat a^\dag\hat a)+\hat a^\dag\hat a=2\hat a^\dag\hat a+1
\tag{2}
\end{equation*}

Substitute (2) into (1) to obtain
\begin{equation*}
\hat H=\hbar\omega\left(\hat a^\dag\hat a+\frac{1}{2}\right)
+\lambda\left(\frac{\hbar}{2m\omega}\left(2\hat a^\dag\hat a+1\right)\right)^2
\end{equation*}

Rewrite using the number operator $\hat n=\hat a^\dag\hat a$.
\begin{equation*}
\hat H=\hbar\omega\left(\hat n+\frac{1}{2}\right)
+\lambda\left(\frac{\hbar}{2m\omega}\left(2\hat n+1\right)\right)^2
\end{equation*}

Expand the quadratic term.
\begin{equation*}
\hat H=\hbar\omega\left(\hat n+\frac{1}{2}\right)
+\lambda\left(\frac{\hbar}{m\omega}\right)^2\left(\hat n^2+\hat n+\frac{1}{4}\right)
\end{equation*}

Hence
\begin{equation*}
\hat H\vert n\rangle
=\hbar\omega\left(n+\frac{1}{2}\right)\vert n\rangle
+\lambda\left(\frac{\hbar}{m\omega}\right)^2\left(n^2+n+\frac{1}{4}\right)\vert n\rangle
\end{equation*}

\end{document}
