\documentclass[12pt]{article}
\usepackage{amsmath}
\parindent=0pt
\begin{document}

(1.4)
Show that
\begin{equation*}
\frac{\delta\phi(x)}{\delta\phi(y)}=\delta(x-y)
\tag{1.44}
\end{equation*}
and
\begin{equation*}
\frac{\delta\dot\phi(t)}{\delta\phi(t_0)}=\frac{d}{dt}\delta(t-t_0)
\tag{1.45}
\end{equation*}

\bigskip
\hrule

\bigskip
Let $F$ be the trivial functional $F[\phi]=\phi(x)$.
\begin{equation*}
\frac{\delta F}{\delta\phi(y)}
=\lim_{\epsilon\rightarrow0}
\frac{\phi(x)+\epsilon\delta(x-y)-\phi(x)}{\epsilon}
=\delta(x-y)
\end{equation*}

Show (1.45).
\begin{equation*}
\frac{\delta\dot\phi(t)}{\delta\phi(t_0)}
=\lim_{\epsilon\rightarrow0}\frac{1}{\epsilon}
\left(
\frac{d\big(\phi(t)-\epsilon\delta(t-t_0)\big)}{dt}-\frac{d\phi(t)}{dt}
\right)
=\frac{d}{dt}\delta(x-y)
\end{equation*}

\end{document}
