\documentclass[12pt]{article}
\usepackage{amsmath}
\parindent=0pt
\begin{document}

(1.6)
Show that if $Z_0[J]$ is given by
\begin{equation*}
Z_0[J]=\exp\left(
-\frac{1}{2}\int d^4x\,d^4y\,J(x)\Delta(x-y)J(y)
\right)
\tag{1.49}
\end{equation*}
where $\Delta(x)=\Delta(-x)$ then
\begin{equation*}
\frac{\delta Z_0[J]}{\delta J(z_1)}
=-\left[
\int d^4y\,\Delta(z_1-y)J(y)
\right]Z_0[J]
\tag{1.50}
\end{equation*}

\bigskip
\hrule

\bigskip
Let
\begin{equation*}
I=\int d^4x\,d^4y\,
\big(J(x)+\epsilon\delta(x-z_1)\big)
\Delta(x-y)
\big(J(y)+\epsilon\delta(y-z_1)\big)
\end{equation*}

Then
\begin{equation*}
\frac{\delta Z_0[J]}{\delta J(z_1)}=\lim_{\epsilon\rightarrow0}
\frac{\exp(-I/2)-Z_0[J]}{\epsilon}
\tag{1}
\end{equation*}

Expand the integrand of $I$ to obtain
\begin{equation*}
I=I_1+\epsilon I_2+\epsilon I_3+\epsilon^2 I_4
\end{equation*}
where
\begin{align*}
I_1&=\int d^4x\,d^4y\,J(x)\Delta(x-y)J(y)
\\
I_2&=\int d^4x\,d^4y\,\delta(x-z_1)\Delta(x-y)J(y)=\int d^4y\,\Delta(z_1-y)J(y)
\\
I_3&=\int d^4x\,d^4y\,J(x)\Delta(x-y)\delta(y-z_1)=\int d^4x\,\Delta(x-z_1)J(x)
\\
I_4&=\int d^4x\,d^4y\,\delta(x-z_1)\Delta(x-y)\delta(y-z_1)=\Delta(0)
\end{align*}

Noting that $\Delta(x-y)=\Delta(y-x)$ we have
\begin{equation*}
I_2+I_3=2I_2
\end{equation*}

The product $\epsilon^2I_4$ vanishes in the limit hence
\begin{equation*}
I=I_1+2\epsilon I_2
\tag{2}
\end{equation*}

Substitute (2) into (1) to obtain
\begin{equation*}
\frac{\delta Z_0[J]}{\delta J(z_1)}=\lim_{\epsilon\rightarrow0}
\frac{\exp(-I_1/2-\epsilon I_2)-Z_0[J]}{\epsilon}
\end{equation*}

Let $X=I_1/2$ and $\epsilon=h/I_2$.
Then
\begin{equation*}
\frac{\delta Z_0[J]}{\delta J(z_1)}=I_2\lim_{h\rightarrow0}
\frac{\exp(-X-h)-\exp(-X)}{h}
=-I_2\exp(-X)
\end{equation*}

Hence
\begin{equation*}
\frac{\delta Z_0[J]}{\delta J(z_1)}=-\left(\int d^4y\,\Delta(z_1-y)J(y)\right)Z_0[J]
\end{equation*}

\end{document}
