\documentclass[12pt]{article}
\usepackage{amsmath}
\parindent=0pt
\begin{document}

(5.2)
Show that Poisson brackets anticommute
\begin{equation*}
\{A,B\}_\mathrm{PB}=-\{B,A\}_\mathrm{PB}
\tag{5.59}
\end{equation*}
and also satisfy the Jacobi identity
\begin{equation*}
\left\{\{A,B\}_\mathrm{PB},C\right\}_\mathrm{PB}
+\left\{\{C,A\}_\mathrm{PB},B\right\}_\mathrm{PB}
+\left\{\{B,C\}_\mathrm{PB},A\right\}_\mathrm{PB}
=0
\tag{5.60}
\end{equation*}
and show that quantum mechanical commutators
also have the same properties.

\bigskip
\hrule

\bigskip
From equation (5.11)
\begin{equation*}
\{A,B\}_\mathrm{PB}
=\frac{\partial A}{\partial q_i}\frac{\partial B}{\partial p_i}
-\frac{\partial A}{\partial p_i}\frac{\partial B}{\partial q_i}
\tag{5.11}
\end{equation*}

Hence
\begin{multline*}
\left\{\{A,B\}_\mathrm{PB},C\right\}_\mathrm{PB}
\\
{}=\frac{\partial}{\partial q_i}
\left(
\frac{\partial A}{\partial q_i}\frac{\partial B}{\partial p_i}
-\frac{\partial A}{\partial p_i}\frac{\partial B}{\partial q_i}
\right)
\frac{\partial C}{\partial p_i}
-\frac{\partial}{\partial p_i}
\left(
\frac{\partial A}{\partial q_i}\frac{\partial B}{\partial p_i}
-\frac{\partial A}{\partial p_i}\frac{\partial B}{\partial q_i}
\right)
\frac{\partial C}{\partial q_i}
\end{multline*}

Eigenmath proof
\begin{verbatim}
PB(f,g) = d(f,q) d(g,p) - d(f,p) d(g,q)

A = a(p,q)
B = b(p,q)
C = c(p,q)

PB(PB(A,B),C) + PB(PB(C,A),B) + PB(PB(B,C),A) == 0
\end{verbatim}

\end{document}
