\documentclass[12pt]{article}
\usepackage{amsmath}
\parindent=0pt
\begin{document}

(8.1)
Show that the form of the time evolution operator
$\hat U(t_2,t_1)=\exp[-i\hat H(t_2-t_1)]$ (as given in eqn 8.7)
exhibits properties 1--5 in Section 8.1.

\bigskip
\hrule

\bigskip
(1) $\hat U(t_1,t_1)=1$

(2) $\hat U(t_3,t_2)\hat U(t_2,t_1)=\hat U(t_3,t_1)$

(3) $i\frac{d}{dt_2}\hat U(t_2,t_1)=\hat H\hat U(t_2,t_1)$

(4) $\hat U(t_1,t_2)=\hat U^{-1}(t_2,t_1)$

(5) $\hat U^\dag(t_2,t_1)\hat U(t_2,t_1)=1$

\bigskip
(1)
\begin{align*}
\hat U(t_1,t_1)
&=\exp[-i\hat H(t_1-t_1)]
\\
&=\exp(0)
\\
&=1
\end{align*}

(2)
\begin{align*}
\hat U(t_3,t_2)\hat U(t_2,t_1)
&=\exp[-i\hat H(t_3-t_2)]\exp[-i\hat H(t_2-t_1)]
\\
&=\exp[-i\hat H(t_3-t_1)]
\\
&=\hat U(t_3,t_1)
\end{align*}

(3)
\begin{align*}
i\frac{d}{dt_2}\hat U(t_2,t_1)
&=i\frac{d}{dt_2}\exp[-i\hat H(t_2-t_1)]
\\
&=i(-i\hat H)\exp[-i\hat H(t_2-t_1)]
\\
&=\hat H\hat U(t_2,t_1)
\end{align*}

(4)
\begin{align*}
\hat U(t_1,t_2)
&=\exp[-i\hat H(t_1-t_2)]
\\
&=\exp[i\hat H(t_2-t_1)]
\\
&=\exp[-i\hat H(t_2-t_1)]^{-1}
\\
&=\hat U^{-1}(t_2,t_1)
\end{align*}

(5)
\begin{align*}
\hat U^\dag(t_2,t_1)\hat U(t_2,t_1)
&=\exp[-i\hat H(t_2-t_1)]^{-1}\exp[-i\hat H(t_2-t_1)]
\\
&=\exp[i\hat H(t_2-t_1)]\exp[-i\hat H(t_2-t_1)]
\\
&=\exp(0)
\\
&=1
\end{align*}

\end{document}
