\documentclass[12pt]{article}
\usepackage{amsmath}
\parindent=0pt
\begin{document}

(3.2)
Show that for the simple harmonic oscillator:

\bigskip
(a) $\left[\hat a,(\hat a^\dag)^n\right]=n(\hat a^\dag)^{n-1}$,

(b) $\langle0|\hat a^n(\hat a^\dag)^m|0\rangle=n!\delta_{nm}$,

(c) $\langle m|\hat a^\dag|n\rangle=\sqrt{n+1}\delta_{m,n+1}$,

(d) $\langle m|\hat a|n\rangle=\sqrt{n}\delta_{m,n-1}$.

\bigskip
\hrule

\bigskip
(a) We have for $r=m+n-1$
\begin{align*}
\left[\hat a,(\hat a^\dag)^n\right]|m\rangle
&=\hat a(\hat a^\dag)^n|m\rangle-(\hat a^\dag)^n\hat a|m\rangle
\\
&=\sqrt{m+n}\left(\prod_{k=1}^n\sqrt{m+k}\right)|r\rangle
-\left(\prod_{k=1}^n\sqrt{m-1+k}\right)\sqrt{m}|r\rangle
\end{align*}

It follows that
\begin{equation*}
\left[\hat a,(\hat a^\dag)^n\right]|m\rangle
=(m+n)\left(\prod_{k=1}^{n-1}\sqrt{m+k}\right)|r\rangle
-m\left(\prod_{k=2}^n\sqrt{m-1+k}\right)|r\rangle
\end{equation*}

Noting that
\begin{equation*}
\prod_{k=1}^{n-1}\sqrt{m+k}=\prod_{k=2}^n\sqrt{m-1+k}
\end{equation*}
we have
\begin{equation*}
\left[\hat a,(\hat a^\dag)^n\right]|m\rangle
=n\left(\prod_{k=1}^{n-1}\sqrt{m+k}\right)|m+n-1\rangle
\end{equation*}

Hence
\begin{equation*}
\left[\hat a,(\hat a^\dag)^n\right]|m\rangle=n(\hat a^\dag)^{n-1}|m\rangle
\end{equation*}


\end{document}
