\documentclass[12pt]{article}
\usepackage{amsmath}
\parindent=0pt
\begin{document}

(14.1)
Fill in the algebra leading to eqn 14.32.

\bigskip
\hrule

\bigskip
Consider equation (14.31).
\begin{equation*}
\hat A^\mu(x)=\int\frac{d^3p}{(2\pi)^\frac{3}{2}}\frac{1}{(2E_p)^\frac{1}{2}}
\sum_{\lambda=1}^2
\left(
\epsilon_\lambda^\mu(p)\hat a_{p\lambda}\exp(-ip\cdot x)
+\epsilon_\lambda^{\mu*}(p)\hat a_{p\lambda}^\dag\exp(ip\cdot x)
\right)
\tag{14.31}
\end{equation*}

Let
\begin{equation*}
\hat A^\mu=\begin{pmatrix}\hat A_0\\\hat A_1\\\hat A_2\\\hat A_3\end{pmatrix},
\qquad
\epsilon_\lambda^\mu(p)=\begin{pmatrix}
\epsilon_{0,p\lambda}\\\epsilon_{1,p\lambda}\\\epsilon_{2,p\lambda}\\\epsilon_{3,p\lambda}
\end{pmatrix}
\end{equation*}

Then in vector form we have
\begin{equation*}
\begin{pmatrix}\hat A_0\\\hat A_1\\\hat A_2\\\hat A_3\end{pmatrix}
=\int\frac{d^3p}{(2\pi)^\frac{3}{2}}\frac{\hat a}{(2E_p)^\frac{1}{2}}
\end{equation*}
where
\begin{multline*}
\hat a=\begin{pmatrix}\epsilon_{0,p1}\\\epsilon_{1,p1}\\\epsilon_{2,p1}\\\epsilon_{3,p1}\end{pmatrix}
\hat a_{p1}\exp(-ip\cdot x)
+\begin{pmatrix}\epsilon_{0,p1}^*\\\epsilon_{1,p1}^*\\\epsilon_{2,p1}^*\\\epsilon_{3,p1}^*\end{pmatrix}
\hat a_{p1}^\dag\exp(ip\cdot x)
\\
{}+\begin{pmatrix}\epsilon_{0,p2}\\\epsilon_{1,p2}\\\epsilon_{2,p2}\\\epsilon_{3,p2}\end{pmatrix}
\hat a_{p2}\exp(-ip\cdot x)
+\begin{pmatrix}\epsilon_{0,p2}^*\\\epsilon_{1,p2}^*\\\epsilon_{2,p2}^*\\\epsilon_{3,p2}^*\end{pmatrix}
\hat a_{p2}^\dag\exp(ip\cdot x)
\end{multline*}

Hence
\begin{multline*}
\hat A_\nu=\int\frac{d^3p}{(2\pi)^\frac{3}{2}}\frac{1}{(2E_p)^\frac{1}{2}}
\\
{}\times
\left[
(\epsilon_{\nu,p1}\hat a_{p1}+\epsilon_{\nu,p2}\hat a_{p2})\exp(-ip\cdot x)
+(\epsilon_{\nu,p1}^*\hat a_{p1}^\dag+\epsilon_{\nu,p2}^*\hat a_{p2}^\dag)\exp(ip\cdot x)
\right]
\end{multline*}

Recall that
\begin{equation*}
p\cdot x=E_pt-p_1x_1-p_2x_2-p_3x_3
\end{equation*}

Hence the partial derivative of $\hat A_\nu$ is
\begin{multline*}
\partial_\mu\hat A_\nu=\int\frac{d^3p}{(2\pi)^\frac{3}{2}}\frac{1}{(2E_p)^\frac{1}{2}}
\\
{}\times
\left[
-ip_\mu(\epsilon_{\nu,p1}\hat a_{p1}+\epsilon_{\nu,p2}\hat a_{p2})\exp(-ip\cdot x)
+ip_\mu(\epsilon_{\nu,p1}^*\hat a_{p1}^\dag+\epsilon_{\nu,p2}^*\hat a_{p2}^\dag)\exp(ip\cdot x)
\right]
\end{multline*}

Consider equation (14.28).
\begin{equation*}
\mathcal H=\frac{1}{2}(\mathbf E^2+\mathbf B^2)
\tag{14.28}
\end{equation*}

We need to integrate Hamiltonian density $\mathcal H$ to obtain $\hat H$, that is,
\begin{equation*}
\hat H=\int d^3x\,\mathcal H
\tag{1}
\end{equation*}

Substitute (14.28) into (1).
\begin{equation*}
\hat H=\frac{1}{2}\int d^3x\,\left(E_1^2+E_2^2+E_3^2+B_1^2+B_2^2+B_3^2\right)
\end{equation*}

From equations (5.28) and (5.29) we have
\begin{equation*}
\mathbf E=\begin{pmatrix}
\partial_0A_1-\partial_1A_0
\\
\partial_0A_2-\partial_2A_0
\\
\partial_0A_3-\partial_3A_0
\end{pmatrix},
\qquad
\mathbf B=\begin{pmatrix}
\partial_3A_2-\partial_2A_3
\\
\partial_1A_3-\partial_3A_1
\\
\partial_2A_1-\partial_1A_2
\end{pmatrix}
\end{equation*}

Start with $E_1^2$.
\begin{equation*}
E_1^2=(\partial_0\hat A_1)^2
-(\partial_0\hat A_1)(\partial_1\hat A_0)
-(\partial_1\hat A_0)(\partial_0\hat A_1)
+(\partial_1\hat A_0)^2
\end{equation*}

Let
\begin{equation*}
I_1=\frac{1}{2}\int d^3x\,(\partial_0\hat A_1)^2
\end{equation*}

Hence
\begin{align*}
I_1&=\frac{1}{2}\int
\frac{d^3x\,d^3p\,d^3q}{(2\pi)^3}\frac{1}{(2E_p)^\frac{1}{2}(2E_q)^\frac{1}{2}}
\\
&\qquad
{}\times\sum_{\lambda=1}^2
\left(
-iE_p\epsilon_\lambda^1(p)\hat a_{p\lambda}\exp(-ip\cdot x)
+iE_p\epsilon_\lambda^{1*}(p)\hat a_{p\lambda}^\dag\exp(ip\cdot x)
\right)
\\
&\qquad
{}\times\sum_{\lambda=1}^2
\left(
-iE_q\epsilon_\lambda^1(q)\hat a_{q\lambda}\exp(-iq\cdot x)
+iE_q\epsilon_\lambda^{1*}(q)\hat a_{q\lambda}^\dag\exp(iq\cdot x)
\right)
\end{align*}

Using the integral
\begin{equation*}
\int d^3x\,\exp(ip\cdot x)=(2\pi)^3\exp(iE_pt)\delta^{(3)}(\mathbf p)
\end{equation*}
we have
\begin{align*}
I_1&=\frac{1}{2}\int
\frac{d^3p\,d^3q}{(2E_p)^\frac{1}{2}(2E_q)^\frac{1}{2}}
\\
&\qquad
{}\times
\delta^{(3)}(\mathbf p)
\sum_{\lambda=1}^2
\left(
-iE_p\epsilon_\lambda^1(p)\hat a_{p\lambda}\exp(-iE_pt)
+iE_p\epsilon_\lambda^{1*}(p)\hat a_{p\lambda}^\dag\exp(iE_pt)
\right)
\\
&\qquad
{}\times
\delta^{(3)}(\mathbf q)
\sum_{\lambda=1}^2
\left(
-iE_q\epsilon_\lambda^1(q)\hat a_{q\lambda}\exp(-iE_qt)
+iE_q\epsilon_\lambda^{1*}(q)\hat a_{q\lambda}^\dag\exp(iE_qt)
\right)
\end{align*}

% FIXME incomplete and some parts are wrong

\end{document}
