\documentclass[12pt]{article}
\usepackage{amsmath}
\parindent=0pt
\begin{document}

(8.2)
For the Hamiltonian
\begin{equation*}
\hat H=\sum_kE_k\hat a_k^\dag\hat a_k
\tag{8.21}
\end{equation*}
use the Heisenberg equation of motion to show that
the time dependence of the operator $\hat a_k^\dag$ is given by
\begin{equation*}
\hat a_k^\dag(t)=\hat a_k^\dag(0)\exp\left(\frac{iE_kt}{\hbar}\right)
\tag{8.22}
\end{equation*}
and find a similar expression for $\hat a_k(t)$.

\bigskip
\hrule

\bigskip
The Heisenberg equation of motion is
\begin{equation*}
\frac{d}{dt}\hat a^\dag(t)=-\frac{i}{\hbar}\left[\hat a^\dag(t),\hat H\right]
\tag{8.15}
\end{equation*}

Substitute (8.22) into the right-hand side of (8.15) and call it $I$.
\begin{equation*}
I=-\frac{i}{\hbar}\exp\left(\frac{iE_kt}{\hbar}\right)
\left(\hat a_k^\dag(0)\hat H-\hat H\hat a_k^\dag(0)\right)
\tag{1}
\end{equation*}

Rewrite the Hamiltonian in equation (8.21) as
\begin{equation*}
\hat H=\sum_jE_j\hat n_j
\tag{2}
\end{equation*}

Substitute (2) into (1). Note that $\hat H$ commutes with $\hat a_k^\dag(0)$ for $j\ne k$.
\begin{equation*}
I=-\frac{i}{\hbar}E_k\exp\left(\frac{iE_kt}{\hbar}\right)
\left(\hat a_k^\dag(0)\hat n_k-\hat n_k\hat a_k^\dag(0)\right)
\end{equation*}

Note that
\begin{equation*}
\hat n\hat a^\dag|n\rangle=(n+1)|n+1\rangle=(n+1)\hat a^\dag|n\rangle
\end{equation*}
and
\begin{equation*}
\hat a\hat n|n\rangle=n|n+1\rangle=n\hat a^\dag|n\rangle
\end{equation*}

Hence
\begin{align*}
I&=-\frac{i}{\hbar}E_k\exp\left(\frac{iE_kt}{\hbar}\right)
\left(\hat n_k\hat a_k^\dag(0)-(\hat n_k+1)\hat a_k^\dag(0)\right)
\\
&=\frac{i}{\hbar}E_k\exp\left(\frac{iE_kt}{\hbar}\right)\hat a_k^\dag(0)
\\
&=\frac{i}{\hbar}E_k\hat a_k^\dag(t)
\tag{3}
\end{align*}

Substitute (8.22) into the left-hand side of (8.15) to obtain
\begin{equation*}
\frac{d}{dt}\hat a^\dag(t)=\frac{i}{\hbar}E_k\hat a_k^\dag(t)
\tag{4}
\end{equation*}

By the equivalence of (3) and (4) we have
\begin{equation*}
\frac{d}{dt}\hat a^\dag(t)=-\frac{i}{\hbar}\left[\hat a^\dag(t),\hat H\right]
\end{equation*}
for the $\hat a^\dag(t)$ given in (8.22).

\bigskip
Because the number operator is time-independent we must have
\begin{equation*}
\hat a_k(t)=\hat a_k(0)\exp\left(-\frac{iE_kt}{\hbar}\right)
\end{equation*}
so that
\begin{equation*}
\hat a_k^\dag(t)\hat a_k(t)=\hat a_k^\dag(0)\hat a_k(0)
\end{equation*}

\end{document}
