\documentclass[12pt]{article}
\usepackage{amsmath}
\parindent=0pt
\begin{document}

(5.3)
Show that the commutator of two Hermitian operators
$\hat A$ and $\hat B$ is anti-Hermitian, i.e., that
\begin{equation*}
[\hat A,\hat B]^\dag=-[\hat A,\hat B]
\tag{5.61}
\end{equation*}

The factor of $i$ in many commutator expressions
(e.g.~$[\hat x,\hat p]=i\hbar$,
$[\hat L_x,\hat L_y]=i\hbar\hat L_z$, and
$[\hat A,\hat B]=\frac{1}{i\hbar}\{A,B\}_\mathrm{PB}$)
makes sure that this property is obeyed.

\bigskip
\hrule

\bigskip
We have
\begin{align*}
[\hat A,\hat B]^\dag
&=(\hat A\hat B-\hat B\hat A)^\dag
\\
&=(\hat A\hat B)^\dag-(\hat B\hat A)^\dag
\\
&=\hat B^\dag\hat A^\dag-\hat A^\dag\hat B^\dag
\end{align*}

Then by Hermiticity
\begin{align*}
\hat B^\dag\hat A^\dag-\hat A^\dag\hat B^\dag
&=\hat B\hat A-\hat A\hat B
\\
&=-[\hat A,\hat B]
\end{align*}

\end{document}
