\documentclass[12pt]{article}
\usepackage{amsmath}
\parindent=0pt
\begin{document}

(2.1)
For the one-dimensional harmonic oscillator, show
that with creation and annihilation operators defined
as in eqns 2.9 and 2.10, $[\hat a,\hat a]=0$,
$[\hat a^\dag,\hat a^\dag]=0$,
$[\hat a,\hat a^\dag]=1$ and
$\hat H=\hbar\omega\left(\hat a^\dag\hat a+\tfrac{1}{2}\right)$.

\bigskip
\hrule

\bigskip
\begin{align*}
\hat a&=\sqrt{\frac{m\omega}{2\hbar}}
\left(\hat x+\frac{i}{m\omega}\hat p\right)
\tag{2.9}
\\
\hat a^\dag&=\sqrt{\frac{m\omega}{2\hbar}}
\left(\hat x-\frac{i}{m\omega}\hat p\right)
\tag{2.10}
\end{align*}

We have by elementary algebra
\begin{equation*}
[\hat a,\hat a]=\hat a\hat a-\hat a\hat a=0
\qquad
[\hat a^\dag,\hat a^\dag]=\hat a^\dag\hat a^\dag-\hat a^\dag\hat a^\dag=0
\end{equation*}

For the commutator $[\hat a,\hat a^\dag]$ we have
\begin{align*}
\hat a\hat a^\dag
&=\frac{m\omega}{2\hbar}
\left(
\hat x\left(\hat x-\frac{i}{m\omega}\hat p\right)
+\frac{i}{m\omega}\hat p\left(\hat x-\frac{i}{m\omega}\hat p\right)
\right)
\\
&=\frac{m\omega}{2\hbar}
\left(
\hat x^2-\frac{i}{m\omega}\hat x\hat p+\frac{i}{m\omega}\hat p\hat x+\frac{1}{m^2\omega^2}\hat p^2\right)
\end{align*}

Rewrite as
\begin{equation*}
\hat a\hat a^\dag
=\frac{m\omega}{2\hbar}\hat x^2-\frac{i}{2\hbar}[\hat x,\hat p]+\frac{1}{2\hbar m\omega}\hat p^2
\end{equation*}

From page 20 just below equation (2.8) we have
\begin{equation*}
[\hat x,\hat p]=i\hbar
\end{equation*}

It follows that
\begin{equation*}
\hat a\hat a^\dag
=\frac{m\omega}{2\hbar}\hat x^2+\frac{1}{2\hbar m\omega}\hat p^2+\frac{1}{2}
\tag{1}
\end{equation*}

By similar argument
\begin{equation*}
\hat a^\dag\hat a
=\frac{m\omega}{2\hbar}\hat x^2+\frac{1}{2\hbar m\omega}\hat p^2-\frac{1}{2}
\tag{2}
\end{equation*}

Hence
\begin{equation*}
[\hat a,\hat a^\dag]=\hat a\hat a^\dag-\hat a^\dag\hat a=\frac{1}{2}-\left(-\frac{1}{2}\right)=1
\end{equation*}

Multiply equation (2) by $\omega\hbar$ to obtain
\begin{equation*}
\omega\hbar\left(\hat a^\dag\hat a\right)=\frac{m\omega^2}{2}\hat x^2+\frac{1}{2m}\hat p^2-\frac{\omega\hbar}{2}
\end{equation*}

Rewrite as
\begin{equation*}
\omega\hbar\left(\hat a^\dag\hat a+\tfrac{1}{2}\right)
=\frac{m\omega^2}{2}\hat x^2+\frac{1}{2m}\hat p^2
\tag{3}
\end{equation*}

Consider equation (2.6).
\begin{equation*}
\hat H=\frac{\hat p^2}{2m}+\frac{1}{2}m\omega^2\hat x^2
\tag{2.6}
\end{equation*}

Substitute (3) into (2.6).
\begin{equation*}
\hat H=\omega\hbar\left(\hat a^\dag\hat a+\tfrac{1}{2}\right)
\end{equation*}

\end{document}
