\documentclass[12pt]{article}
\usepackage{amsmath}
\parindent=0pt
\begin{document}

(1.3)
Consider the functional $G[f]=\int g(y,f)\,dy$.
Show that
\begin{equation*}
\frac{\delta G[f]}{\delta f(x)}=\frac{\partial g(x,f)}{\partial f}
\tag{1.41}
\end{equation*}

Now consider the functional $H[f]=\int g(y,f,f')\,dy$
and show that
\begin{equation*}
\frac{\delta H[f]}{\delta f(x)}=\frac{\partial g}{\partial f}
-\frac{d}{dx}\frac{\partial g}{\partial f'}
\tag{1.42}
\end{equation*}
where $f'=\partial f/\partial y$.
For the functional $J[f]=\int g(y,f,f',f'')\,dy$ show that
\begin{equation*}
\frac{\delta J[f]}{\delta f(x)}
=\frac{\partial g}{\partial f}
-\frac{d}{dx}\frac{\partial g}{\partial f'}
+\frac{d^2}{dx^2}\frac{\partial g}{\partial f''}
\tag{1.43}
\end{equation*}
where $f''=\partial^2 f/\partial y^2$.

\bigskip
\hrule

\bigskip
To show (1.41) we start with
\begin{equation*}
\frac{\delta G[f]}{\delta f(x)}
=\lim_{\epsilon\rightarrow 0}\left(
\int g\big(y,f+\epsilon\delta(y-x)\big)\,dy-\int g(y,f)\,dy
\right)
\end{equation*}

By Taylor series expansion (higher powers of $\epsilon$ vanish in the limit)
\begin{equation*}
\frac{\delta G[f]}{\delta f(x)}
=\lim_{\epsilon\rightarrow 0}
\left(
\int g(y,f)\,dy
+\int\epsilon\delta(y-x)\frac{\partial g(y,f)}{\partial f}\,dy
-\int g(y,f)\,dy
\right)
\end{equation*}

Hence
\begin{equation*}
\frac{\delta G[f]}{\delta f(x)}=\frac{\partial g(x,f)}{\partial f}
\end{equation*}

Now show (1.42).
Let
\begin{equation*}
h=f+\epsilon\delta(y-x)
\qquad
h'=\frac{\partial h}{\partial y}
\end{equation*}

Then
\begin{equation*}
\frac{\delta H[f]}{\delta f(x)}
=\lim_{\epsilon\rightarrow 0}
\left(
\int g(y,h,h')\,dy-\int g(y,f)\,dy
\right)
\end{equation*}

Taylor expand the first integrand up to linear powers of $\epsilon$.
\begin{equation*}
g(y,h,h')=g(y,f,f')
+\epsilon\delta(y-x)\frac{\partial g(y,f,f')}{\partial f}
+\epsilon\frac{\partial\delta(y-x)}{\partial y}\frac{\partial g(y,f,f')}{\partial f'}
\end{equation*}

Hence
\begin{equation*}
\frac{\delta H[f]}{\delta f(x)}
=\int\delta(y-x)\frac{\partial g(y,f,f')}{\partial f}\,dy
+\int\frac{\partial\delta(y-x)}{\partial y}\frac{\partial g(y,f,f')}{\partial f'}\,dy
\tag{1}
\end{equation*}

The first integral is solved by (1.41).
\begin{equation*}
\int\delta(y-x)\frac{\partial g(y,f,f')}{\partial f}\,dy
=\frac{\partial g(x,f,f')}{\partial f}
\tag{2}
\end{equation*}

For the second integral, let
\begin{equation*}
u=\frac{\partial g(y,f,f')}{\partial f'}
\qquad
v=\delta(y-x)
\end{equation*}

Then
\begin{equation*}
du=\frac{\partial}{\partial y}\frac{\partial g(y,f,f')}{\partial f'}\,dy
\qquad
dv=\frac{\partial\delta(y-x)}{\partial y}\,dy
\end{equation*}
and
\begin{equation*}
\int\frac{\partial\delta(y-x)}{\partial y}\frac{\partial g(y,f,f')}{\partial f'}\,dy
=\int u\,dv
\end{equation*}

Integrate by parts.
\begin{align*}
&\int\frac{\partial\delta(y-x)}{\partial y}\frac{\partial g(y,f,f')}{\partial f'}\,dy
\\
&\qquad{}=uv-\int v\,du
\\
&\qquad{}=\frac{\partial g(y,f,f')}{\partial f'}\delta(y-x)
-\int\delta(y-x)\frac{\partial}{\partial y}\frac{\partial g(y,f,f')}{\partial f'}\,dy
\\
&\qquad{}=-\frac{\partial}{\partial x}\frac{\partial g(x,f,f')}{\partial f'}
\tag{3}
\end{align*}

Substitute (2) and (3) into (1) to obtain (1.42).
\begin{equation*}
\frac{\delta H[f]}{\delta f(x)}
=\frac{\partial g(x,f,f')}{\partial f}
-\frac{\partial}{\partial x}\frac{\partial g(x,f,f')}{\partial f'}
\end{equation*}

\end{document}
