\documentclass[12pt]{article}
\usepackage{amsmath}
\parindent=0pt
\begin{document}

(9.1)
Deduce that the generators of the translation operator
are given by
\begin{equation*}
\hat{\mathbf p}=-\frac{1}{i}
\frac{\partial\hat U(\mathbf a)}{\partial\mathbf a}\bigg|_{\mathbf a=0}
\tag{9.51}
\end{equation*}

\bigskip
\hrule

\bigskip
From page 81 we have
\begin{equation*}
\hat U(\mathbf a)=\exp(-i\hat{\mathbf p}\cdot\mathbf a)
\end{equation*}

Hence
\begin{equation*}
\frac{\partial\hat U(\mathbf a)}{\partial\mathbf a}=-i\hat{\mathbf p}\exp(-i\hat{\mathbf p}\cdot\mathbf a)
\end{equation*}

Then for $\mathbf a=0$ we have
\begin{equation*}
\frac{\partial\hat U(\mathbf a)}{\partial\mathbf a}=-i\hat{\mathbf p}
\end{equation*}

\end{document}
