\documentclass[12pt]{article}
\usepackage{amsmath}
\parindent=0pt
\begin{document}

(2.4)
Using $\hat a|0\rangle=0$ and eqns 2.9 and 2.10 together with
$\langle x|\hat p|\psi\rangle=-i\hbar\frac{d}{dx}\langle x|\psi\rangle$, show that
\begin{equation*}
0=\left(x+\frac{\hbar}{m\omega}\frac{d}{dx}\right)
\langle x|0\rangle
\tag{2.69}
\end{equation*}
and hence
\begin{equation*}
\langle x|0\rangle=\left(\frac{m\omega}{\pi\hbar}\right)^{1/4}
\exp\left(-\frac{m\omega x^2}{2\hbar}\right)
\tag{2.70}
\end{equation*}

\bigskip
\hrule

\bigskip
\begin{align*}
\hat a&=\sqrt{\frac{m\omega}{2\hbar}}
\left(\hat x+\frac{i}{m\omega}\hat p\right)
\tag{2.9}
\\
\hat a^\dag&=\sqrt{\frac{m\omega}{2\hbar}}
\left(\hat x-\frac{i}{m\omega}\hat p\right)
\tag{2.10}
\end{align*}

We have
\begin{equation*}
\left(x+\frac{\hbar}{m\omega}\frac{d}{dx}\right)\langle x|0\rangle
=\langle x|\left(\hat x+\frac{i}{m\omega}\hat p\right)|0\rangle
=\langle x|\hat a|0\rangle
=0
\end{equation*}

Let
\begin{equation*}
f=\exp\left(-\frac{m\omega x^2}{2\hbar}\right)
\end{equation*}

Then
\begin{equation*}
\frac{d}{dx}f=-\frac{m\omega x}{\hbar}\exp\left(-\frac{m\omega x^2}{2\hbar}\right)
\end{equation*}

It follows that
\begin{equation*}
\frac{\hbar}{m\omega}\frac{d}{dx}f=-xf
\end{equation*}

Hence (2.70) is a solution to differential equation (2.69).

\end{document}
